Aaaaaaaand back to the start but with a generic typing this time

theories/Escape.v
@@ -6,57 +6,90 @@ Set Universe Polymorphism.
 Section Escapes.
   Context `{GenericTypingProp}.
 
-  Definition escape {l Γ A} :
+  Definition escape {l Γ A eqTy redTm eqTm} :
+    LRl l Γ A eqTy redTm eqTm ->
+    [Γ |- A].
+  Proof.
+    induction 1 as [? [] | ? ? [] | ? ? [] ].
+    all: gen_typing.
+  Qed.
+
+  Corollary escape_ {l Γ A} :
       [Γ ||-< l > A ] ->
       [Γ |- A].
   Proof.
     intros [[] lr].
-    cbn in lr.
-    red in lr.
-    induction lr as [? [] | ? ? [] | ? ? [] ].
-    all: gen_typing.
+    now eapply escape.
   Qed.
 
-  Definition escapeEq {l Γ A B} (lr : [Γ ||-< l > A]) :
-      [ Γ ||-< l > A ≅ B | lr ] ->
-      [Γ |- A ≅ B].
+  Definition escapeEq {l Γ A eqTy redTm eqTm}
+    (lr : LRl l Γ A eqTy redTm eqTm) {B} :
+    eqTy B ->
+    [Γ |- A ≅ B].
   Proof.
-    destruct lr as [[] lr].
-    cbn in *.
     induction lr as [ ? [] | ? ? [] | ? ? [] IHdom IHcod].
     + intros [->].
       gen_typing.
     + intros [].
       cbn in *.
-      gen_typing.
+      eapply convty_exp.
+      all: gen_typing.
     + intros [].
       cbn in *.
       gen_typing.
   Qed.
 
-  Definition escapeTerm {l Γ t A} (lr : [Γ ||-< l > A ]) :
-    [Γ ||-< l > t : A | lr ] ->
+  Corollary escapeEq_ {l Γ A B} (lr : [Γ ||-< l > A]) :
+      [ Γ ||-< l > A ≅ B | lr ] ->
+      [Γ |- A ≅ B].
+  Proof.
+    intros.
+    destruct lr as [[] lr] ; cbn in *.
+    now eapply escapeEq.
+  Qed.
+
+  Definition escapeTerm {l Γ A eqTy redTm eqTm}
+    (lr : LRl l Γ A eqTy redTm eqTm) {t} :
+    redTm t ->
     [Γ |- t : A].
   Proof.
-    destruct lr as [[] lr].
-    cbn in *.
     induction lr as [ ? [] | ? ? [] | ? ? [] IHdom IHcod].
     all: intros [] ; cbn in *.
     all: gen_typing.
+  Qed. 
+
+  Definition escapeTerm_ {l Γ t A} (lr : [Γ ||-< l > A ]) :
+    [Γ ||-< l > t : A | lr ] ->
+    [Γ |- t : A].
+  Proof.
+    intros.
+    destruct lr as [[] lr] ; cbn in *.
+    now eapply escapeTerm.
   Qed.
 
-  Definition escapeEqTerm {l Γ t u A} (lr : [Γ ||-< l > A ]) :
-    [Γ ||-< l > t ≅ u : A | lr ] ->
+  Definition escapeEqTerm {l Γ A eqTy redTm eqTm}
+    (lr : LRl l Γ A eqTy redTm eqTm) {t u} :
+    eqTm t u ->
     [Γ |- t ≅ u : A].
   Proof.
-    destruct lr as [[] lr].
-    cbn in *.
     induction lr as [ ? [] | ? ? [] | ? ? [] IHdom IHcod].
     - intros [[termL] [termR]] ; cbn in *.
-      gen_typing.
+      eapply convtm_exp ; tea.
+      all: gen_typing.
     - intros [] ; cbn in *.
-      eapply convtm_exp.
+      eapply convtm_exp ; tea.
       all: gen_typing.
     - intros [[termL] [termR]] ; cbn in *.
       gen_typing.
   Qed.
+
+  Definition escapeEqTerm_ {l Γ t u A} (lr : [Γ ||-< l > A ]) :
+    [Γ ||-< l > t ≅ u : A | lr ] ->
+    [Γ |- t ≅ u : A].
+  Proof.
+    intros.
+    destruct lr as [[] lr] ; cbn in *.
+    now eapply escapeEqTerm.
+  Qed.
+  
+End Escapes.
