theories/Reflexivity.v
@@ -1,54 +1,52 @@
-From MetaCoq Require Import PCUICAst.
-Require Import Notations Untyped DeclarativeTyping LogicalRelation Properties Reduction LRInduction Escape.
+From MetaCoq Require Import PCUICAst PCUICSigmaCalculus PCUICRenameConv PCUICSigmaCalculus PCUICInstConv.
+Require Import Notations Untyped Weakening GenericTyping DeclarativeTyping LogicalRelation Properties Reduction LRInduction Escape.
 
-Definition LRTyEqRefl {l Γ A eqTy redTm eqTm}
-  (lr : LRl l Γ A eqTy redTm eqTm) : eqTy A.
-Proof.
-  induction lr as [ ? [] | ? ? [] | ? ? [] IHdom IHcod] using LR_rect.
-  + econstructor.
-    reflexivity.
-  + now econstructor.
-  + econstructor.
-    all: mltt.
-Qed.
+Section Reflexivities.
+  Context `{GenericTypingProp}.
 
-Corollary LRTyEqRefl_ {l Γ A} (lr : [ Γ ||-< l > A ] ) : [ Γ ||-< l > A ≅ A | lr ].
-Proof.
-  destruct lr as [[] lr].
-  cbn in *.
-  now eapply LRTyEqRefl.
-Qed.
+  Definition LRTyEqRefl {l Γ A eqTy redTm eqTm}
+    (lr : LRl l Γ A eqTy redTm eqTm) : eqTy A.
+  Proof.
+    induction lr as [ ? [] | ? ? [] | ? ? [] ? IHdom IHcod].
+    all: now econstructor.
+  Qed.
 
-Definition LRTmEqRefl {l Γ A eqTy redTm eqTm} (lr : LRl l Γ A eqTy redTm eqTm) :
-  forall t, redTm t -> eqTm t t.
-Proof.
-  induction lr as [ ? [? []] | ? ? [] | ? ? [] IHdom IHcod] using LR_rect.
-  - intros t [? ? ? [[] rel]] ; cbn in *.
-    assert (eqTy t)
-      by now eapply (LRTyEqRefl (l := zero)).
-    unshelve econstructor.
-    all : cbn.
-    1-2: econstructor ; tea ; cbn.
-    1-3,5: now eapply (LRbuild (l := zero)).
-    all: cbn.
-    all: mltt.
-  - intros t [].
-    econstructor ; cbn in *.
-    1-4: eassumption.
-    eapply TermConv.
-    all: mltt.
-  - intros t [].
-    unshelve econstructor ; cbn in *.
-    1-2: now econstructor.
-    all: cbn.
-    all: mltt.
-Qed.
+  Corollary LRTyEqRefl_ {l Γ A} (lr : [ Γ ||-< l > A ] ) : [ Γ ||-< l > A ≅ A | lr ].
+  Proof.
+    destruct lr as [[] lr].
+    cbn in *.
+    now eapply LRTyEqRefl.
+  Qed.
 
-Definition LREqTermRefl_ {l Γ A t} (lr : [ Γ ||-< l > A ] ) : 
-    [ Γ ||-< l > t : A | lr ] ->
-    [ Γ ||-< l > t ≅ t : A | lr ].
-Proof.
-  destruct lr as [[] lr].
-  cbn in *.
-  now eapply LRTmEqRefl.
-Qed.
+  Definition LRTmEqRefl {l Γ A eqTy redTm eqTm} (lr : LRl l Γ A eqTy redTm eqTm) :
+    forall t, redTm t -> eqTm t t.
+  Proof.
+    induction lr as [ ? [? []] | ? ? [] | ? ? [] IHdom IHcod].
+    - intros t [? ? ? ? [[] rel]] ; cbn in *.
+      assert (eqTy t)
+        by now eapply (LRTyEqRefl (l := zero)).
+      unshelve econstructor.
+      all : cbn.
+      1-2: econstructor ; tea ; cbn.
+      1-3,5: now eapply (LRbuild (l := zero)).
+      all: easy.
+    - intros t [].
+      econstructor ; cbn in *.
+      all: eassumption.
+    - intros t [].
+      unshelve econstructor ; cbn in *.
+      1-2: now econstructor.
+      all: cbn.
+      all: now eauto.
+  Qed.
+
+  Definition LREqTermRefl_ {l Γ A t} (lr : [ Γ ||-< l > A ] ) : 
+      [ Γ ||-< l > t : A | lr ] ->
+      [ Γ ||-< l > t ≅ t : A | lr ].
+  Proof.
+    destruct lr as [[] lr].
+    cbn in *.
+    now eapply LRTmEqRefl.
+  Qed.
+
+End Reflexivities.
