theories/ShapeView.v
@@ -1,83 +1,84 @@
 From MetaCoq Require Import PCUICAst.
-From LogRel Require Import Untyped DeclarativeTyping LogicalRelation Properties Reduction LRInduction Reflexivity.
+From LogRel Require Import Notations Untyped GenericTyping LogicalRelation Properties Reduction LRInduction Reflexivity.
 
 Set Universe Polymorphism.
 
-Definition ShapeView Γ
-  A {lA eqTyA redTmA redTyA} B {lB eqTyB redTmB redTyB}
-  (lrA : LRl lA Γ A eqTyA redTmA redTyA) (lrB : LRl lB Γ B eqTyB redTmB redTyB) : Type :=
-  match lrA, lrB with
-    | LRU _ _, LRU _ _ => True
-    | LRne _ _ _, LRne _ _ _ => True
-    | LRPi _ _ _ _, LRPi _ _ _ _ => True
-    | _, _ => False
-  end.
-  
-  (* | SVU (UredA UredB : [ Γ ||-U l]):
-        ShapeView l Γ U U (LRU (LogRelRec l) UredA) (LRU (LogRelRec l) UredB)
+Section ShapeViews.
+  Context `{GenericTypingProp}.
 
-    | SVne {A B} neA neB :
-        ShapeView l Γ A B (LRne (LogRelRec l) neA) (LRne (LogRelRec l) neB)
+  Definition ShapeView Γ
+    A {lA eqTyA redTmA redTyA} B {lB eqTyB redTmB redTyB}
+    (lrA : LRl lA Γ A eqTyA redTmA redTyA) (lrB : LRl lB Γ B eqTyB redTmB redTyB) : Type :=
+    match lrA, lrB with
+      | LRU _ _, LRU _ _ => True
+      | LRne _ _ _, LRne _ _ _ => True
+      | LRPi _ _ _ _, LRPi _ _ _ _ => True
+      | _, _ => False
+    end.
+    
+    (* | SVU (UredA UredB : [ Γ ||-U l]):
+          ShapeView l Γ U U (LRU (LogRelRec l) UredA) (LRU (LogRelRec l) UredB)
 
-    | SVPi {A B} ΠA ΠB ΠAad ΠBad:
-        ShapeView l Γ A B (LRPi (LogRelRec l) ΠA ΠAad) (LRPi (LogRelRec l) ΠB ΠBad). *)
+      | SVne {A B} neA neB :
+          ShapeView l Γ A B (LRne (LogRelRec l) neA) (LRne (LogRelRec l) neB)
 
-Arguments ShapeView Γ A {lA eqTyA redTmA redTyA} B {lB eqTyB redTmB redTyB}
-!lrA !lrB.
+      | SVPi {A B} ΠA ΠB ΠAad ΠBad:
+          ShapeView l Γ A B (LRPi (LogRelRec l) ΠA ΠAad) (LRPi (LogRelRec l) ΠB ΠBad). *)
 
-Lemma ShapeViewConv {Γ A lA eqTyA redTmA eqTmA B lB eqTyB redTmB eqTmB}
-  (lrA : LRl lA Γ A eqTyA redTmA eqTmA) (lrB : LRl lB Γ B eqTyB redTmB eqTmB) :
-  eqTyA B ->
-  ShapeView Γ A B lrA lrB.
-Proof.
-  destruct lrA.
-  - destruct lrB.
-    + constructor.
-    + intros [->].
-      inversion neA.
-      enough (ty = U) as -> by (now eapply neU).
-      eapply nred_det_ty.
-      all: mltt.
-    + intros [->].
-      inversion ΠA.
-      enough (U = redPi) by (unfold U, redPi in * ; congruence).
-      eapply nred_det_ty.
-      2: mltt.
-      mltt.
-  - destruct lrB.
-    + intros [].
-      inversion neA.
-      enough (ty = U) as -> by (now eapply neU).
-      eapply nred_det_ty.
-      all: mltt.
-    + econstructor.
-    + intros [].
-      destruct ΠA ; cbn in *.
-      enough (ty = redPi) as -> by (now eapply nePi).
-      unfold redPi.
-      eapply nred_det_ty.
-      all: mltt.
-  - destruct lrB.
-    + intros [].
-      inversion ΠA.
-      enough (U = redPi) by (unfold U, redPi in * ; congruence).
-      eapply nred_det_ty.
-      2: mltt.
-      mltt.
-    + intros [].
-      destruct neA.
-      enough (ty = redPi) as -> by now (eapply nePi).
-      unfold redPi.
-      eapply nred_det_ty.
-      all: mltt.
-    + econstructor.
-Qed.
+  Arguments ShapeView Γ A {lA eqTyA redTmA redTyA} B {lB eqTyB redTmB redTyB}
+  !lrA !lrB.
 
-Corollary ShapeViewRefl {Γ A lA eqTyA redTmA eqTmA lA' eqTyA' redTmA' eqTmA'}
-  (lrA : LRl lA Γ A eqTyA redTmA eqTmA) (lrA' : LRl lA' Γ A eqTyA' redTmA' eqTmA') :
-  ShapeView Γ A A lrA lrA'.
-Proof.
-  now eapply ShapeViewConv, LRTyEqRefl.
-Qed.
+  Lemma ShapeViewConv {Γ A lA eqTyA redTmA eqTmA B lB eqTyB redTmB eqTmB}
+    (lrA : LRl lA Γ A eqTyA redTmA eqTmA) (lrB : LRl lB Γ B eqTyB redTmB eqTmB) :
+    eqTyA B ->
+    ShapeView Γ A B lrA lrB.
+  Proof.
+    destruct lrA.
+    - destruct lrB.
+      + constructor.
+      + intros [->].
+        inversion neA.
+        enough (ty = U) as -> by (now eapply neU).
+        symmetry.
+        eapply mredty_whnf.
+        all: gen_typing.
+      + intros [->].
+        inversion ΠA.
+        enough (U = tProd na dom cod) by (unfold U in * ; congruence).
+        eapply mredty_whnf.
+        all: gen_typing.
+    - destruct lrB.
+      + intros [].
+        inversion neA.
+        enough (ty = U) as -> by (now eapply neU).
+        symmetry.
+        eapply mredty_whnf.
+        all: gen_typing.
+      + econstructor.
+      + intros [].
+        destruct ΠA ; cbn in *.
+        enough (ty = tProd na dom cod) as -> by (now eapply nePi).
+        eapply whredty_det.
+        all: gen_typing.
+    - destruct lrB.
+      + intros [].
+        inversion ΠA.
+        enough (U = tProd na dom cod) by (unfold U in * ; congruence).
+        eapply mredty_whnf.
+        all: gen_typing.
+      + intros [].
+        destruct neA.
+        enough (ty = tProd na dom cod) as -> by now (eapply nePi).
+        eapply whredty_det.
+        all: gen_typing.
+      + now easy. 
+  Qed.
 
-Arguments PiRedTy.redPi / Γ A p.
+  Corollary ShapeViewRefl {Γ A lA eqTyA redTmA eqTmA lA' eqTyA' redTmA' eqTmA'}
+    (lrA : LRl lA Γ A eqTyA redTmA eqTmA) (lrA' : LRl lA' Γ A eqTyA' redTmA' eqTmA') :
+    ShapeView Γ A A lrA lrA'.
+  Proof.
+    now eapply ShapeViewConv, LRTyEqRefl.
+  Qed.
+
+End ShapeViews.
